specialize ktcore Sign specs to KT sigpred

proof/ktcore_proof/sigpred.v
@@ -4,16 +4,16 @@ From New.proof.github_com.sanjit_bhat.pav Require Import
   hashchain merkle safemarshal.
 
 From New.proof.github_com.sanjit_bhat.pav.ktcore_proof Require Import
-  ktcore serde.
+  serde.
 
 Module ktcore.
-Import ktcore.ktcore serde.ktcore.
+Import serde.ktcore.
 
 Module sigpred_cfg.
 Record t :=
   mk {
     vrf: gname;
-    startEp: gname;
+    start_ep: gname;
     links: gname;
   }.
 End sigpred_cfg.
@@ -22,22 +22,24 @@ Section proof.
 Context `{hG: heapGS Σ, !ffi_semantics _ _, !globalsGS Σ} {go_ctx : GoContext}.
 Context `{!pavG Σ}.
 
-Definition sigpred_vrf γ enc : iProp Σ :=
+Definition sigpred_vrf γ (vrfPk : list w8) :=
+  "#Hshot" ∷ ghost_var γ.(sigpred_cfg.vrf) (□) vrfPk.
+
+Definition sigpred_vrf_aux γ enc : iProp Σ :=
   ∃ vrfPk,
   "%Henc" ∷ ⌜enc = ktcore.VrfSig.pure_enc (ktcore.VrfSig.mk' (W8 ktcore.VrfSigTag) vrfPk)⌝ ∗
   "%Hvalid" ∷ ⌜safemarshal.Slice1D.valid vrfPk⌝ ∗
+  "#Hsigpred" ∷ sigpred_vrf γ vrfPk.
 
-  "#Hshot" ∷ ghost_var γ (□) vrfPk.
-
-Definition sigpred_links_inv (startEp : w64) links digs cut maps : iProp Σ :=
+Definition sigpred_links_inv (start_ep : w64) links digs cut maps : iProp Σ :=
   (* [offset] is the number of [digs] prior to [links] starting.
-  we leave [digs] un-tied to [startEp], even tho it's implicitly
+  we leave [digs] un-tied to [start_ep], even tho it's implicitly
   constrained by [is_chain]. *)
   let offset := (length digs - length links)%nat in
   "%Hlt_digs_links" ∷ ⌜length links ≤ length digs⌝ ∗
   "#Hlinks" ∷ ([∗ list] idx ↦ link ∈ links,
     let n_digs := (offset + idx + 1)%nat in
-    let ep := (uint.nat startEp + idx)%nat in
+    let ep := (uint.nat start_ep + idx)%nat in
     "#His_link" ∷ hashchain.is_chain (take n_digs digs) cut link (S ep)) ∗
   "#Hmaps" ∷ ([∗ list] idx ↦ _;m ∈ links;maps,
     ∃ dig,
@@ -48,21 +50,23 @@ Definition sigpred_links_inv (startEp : w64) links digs cut maps : iProp Σ :=
     maps !! (S i) = Some m1 →
     m0 ⊆ m1⌝.
 
-Definition sigpred_links γstartEp γlinks enc : iProp Σ :=
-  (* [links] are all audited. they start from [startEp]. *)
-  ∃ ep link startEp links digs cut maps,
+Definition sigpred_links γ (ep : w64) link : iProp Σ :=
+  ∃ start_ep links digs cut maps,
+  (* externalize start_ep so that users agree on the epochs associated with links. *)
+  "#Hshot" ∷ ghost_var γ.(sigpred_cfg.start_ep) (□) start_ep ∗
+  "#Hlb" ∷ mono_list_lb_own γ.(sigpred_cfg.links) links ∗
+  "%Hlook" ∷ ⌜links !! (uint.nat ep - uint.nat start_ep)%nat = Some link⌝ ∗
+  "#Hinv" ∷ sigpred_links_inv start_ep links digs cut maps.
+
+Definition sigpred_links_aux γ enc : iProp Σ :=
+  (* [links] are all audited. they start from [start_ep]. *)
+  ∃ ep link,
   "%Henc" ∷ ⌜enc = ktcore.LinkSig.pure_enc (ktcore.LinkSig.mk' (W8 ktcore.LinkSigTag) ep link)⌝ ∗
   "%Hvalid" ∷ ⌜safemarshal.Slice1D.valid link⌝ ∗
-
-  (* externalize startEp so that users agree on the epochs associated with links. *)
-  "#Hshot" ∷ ghost_var γstartEp (□) startEp ∗
-  "#Hlb" ∷ mono_list_lb_own γlinks links ∗
-  "%Hlook" ∷ ⌜links !! (uint.nat ep - uint.nat startEp)%nat = Some link⌝ ∗
-  "#Hinv" ∷ sigpred_links_inv startEp links digs cut maps.
+  "#Hsigpred" ∷ sigpred_links γ ep link.
 
 Definition sigpred γ enc : iProp Σ :=
-  sigpred_vrf γ.(sigpred_cfg.vrf) enc ∨
-  sigpred_links γ.(sigpred_cfg.startEp) γ.(sigpred_cfg.links) enc.
+  sigpred_vrf_aux γ enc ∨ sigpred_links_aux γ enc.
 
 #[global] Instance sigpred_pers γ e : Persistent (sigpred γ e).
 Proof. apply _. Qed.
